---
heading: Part 3
title: "Theory of the Transformation of Co-ordinates and Times"
weight: 6
date: 2025-01-25
# linkTitle: "EPR Paradox"
# date: 2022-08-08
description: "Einstein explains Relativity"
image: "/covers/electro.jpg"
---


### Theory of the Transformation of Co-ordinates and Times from a Stationary System to another System in
Uniform Motion of Translation Relatively to the Former

Let us in “stationary” space take two systems of co-ordinates, i.e. two sys-
tems, each of three rigid material lines, perpendicular to one another, and issuing
from a point. Let the axes of X of the two systems coincide, and their axes of
Y and Z respectively be parallel. Let each system be provided with a rigid
measuring-rod and a number of clocks, and let the two measuring-rods, and
likewise all the clocks of the two systems, be in all respects alike.
Now to the origin of one of the two systems (k) let a constant velocity v
be imparted in the direction of the increasing x of the other stationary system
(K), and let this velocity be communicated to the axes of the co-ordinates, the
relevant measuring-rod, and the clocks. To any time of the stationary system K
there then will correspond a definite position of the axes of the moving system,
and from reasons of symmetry we are entitled to assume that the motion of k
may be such that the axes of the moving system are at the time t (this “t” always
denotes a time of the stationary system) parallel to the axes of the stationary
system.

We now imagine space to be measured from the stationary system K by
means of the stationary measuring-rod, and also from the moving system k
by means of the measuring-rod moving with it; and that we thus obtain the
co-ordinates x, y, z, and ξ, η, ζ respectively. Further, let the time t of the
stationary system be determined for all points thereof at which there are clocks
by means of light signals in the manner indicated in § 1; similarly let the time
τ of the moving system be determined for all points of the moving system at
which there are clocks at rest relatively to that system by applying the method,
given in § 1, of light signals between the points at which the latter clocks are
located.

To any system of values x, y, z, t, which completely defines the place and
time of an event in the stationary system, there belongs a system of values ξ,
5η, ζ τ , determining that event relatively to the system k, and our task is now
to find the system of equations connecting these quantities.
In the first place it is clear that the equations must be linear on account of
the properties of homogeneity which we attribute to space and time.
If we place x0 = x − vt, it is clear that a point at rest in the system k must
have a system of values x0 , y, z, independent of time. We first define τ as a
function of x0 , y, z, and t. To do this we have to express in equations that τ is
nothing else than the summary of the data of clocks at rest in system k, which
have been synchronized according to the rule given in § 1.

From the origin of system k let a ray be emitted at the time τ0 along the
X-axis to x0 , and at the time τ1 be reflected thence to the origin of the co-
ordinates, arriving there at the time τ2 ; we then must have 12 (τ0 + τ2 ) = τ1 , or,
by inserting the arguments of the function τ and applying the principle of the
constancy of the velocity of light in the stationary system:—





x0
x0
1
x0
0
τ (0, 0, 0, t) + τ 0, 0, 0, t +
+
= τ x , 0, 0, t +
.
2
c−v
c+v
c−v
Hence, if x0 be chosen infinitesimally small,


1
∂τ
1 ∂τ
1
∂τ
1
+
=
,
+
2 c − v c + v ∂t
∂x0
c − v ∂t
or
v
∂τ
∂τ
= 0.
+ 2
0
2
∂x
c − v ∂t
It is to be noted that instead of the origin of the co-ordinates we might have
chosen any other point for the point of origin of the ray, and the equation just
obtained is therefore valid for all values of x0 , y, z.
An analogous consideration—applied to the axes of Y and Z—it being borne
in mind that light is always propagated
√ along these axes, when viewed from the
stationary system, with the velocity c2 − v 2 gives us
∂τ
∂τ
= 0,
= 0.
∂y
∂z
Since τ is a linear function, it follows from these equations that


v
0
τ =a t− 2
x
c − v2
where a is a function φ(v) at present unknown, and where for brevity it is
assumed that at the origin of k, τ = 0, when t = 0.
With the help of this result we easily determine the quantities ξ, η, ζ by
expressing in equations that light (as required by the principle of the constancy
of the velocity of light, in combination with the principle of relativity) is also
6propagated with velocity c when measured in the moving system. For a ray of
light emitted at the time τ = 0 in the direction of the increasing ξ


v
0
ξ = cτ or ξ = ac t − 2
x .
c − v2
But the ray moves relatively to the initial point of k, when measured in the
stationary system, with the velocity c − v, so that
x0
= t.
c−v
If we insert this value of t in the equation for ξ, we obtain
c2
ξ=a 2
x0 .
c − v2
In an analogous manner we find, by considering rays moving along the two other
axes, that


v
0
η = cτ = ac t − 2
x
c − v2
when
y
√
= t, x0 = 0.
2
c − v2
Thus
c
c
η = a√
y and ζ = a √
z.
2
2
2
c −v
c − v2
Substituting for x0 its value, we obtain
τ
ξ=
=φ(v)β(t − vx/c2 ),
φ(v)β(t − vt),
η
ζ=
=φ(v)y,
φ(v)z,
where
1
,
β= p
1 − v 2 /c2
and φ is an as yet unknown function of v. If no assumption whatever be made
as to the initial position of the moving system and as to the zero point of τ , an
additive constant is to be placed on the right side of each of these equations.
7We now have to prove that any ray of light, measured in the moving system,
is propagated with the velocity c, if, as we have assumed, this is the case in the
stationary system; for we have not as yet furnished the proof that the principle
of the constancy of the velocity of light is compatible with the principle of
relativity.

At the time t = τ = 0, when the origin of the co-ordinates is common to the
two systems, let a spherical wave be emitted therefrom, and be propagated with
the velocity c in system K. If (x, y, z) be a point just attained by this wave,
then
x2 + y 2 + z 2 = c2 t2 .
Transforming this equation with the aid of our equations of transformation
we obtain after a simple calculation
ξ 2 + η 2 + ζ 2 = c2 τ 2 .

The wave under consideration is therefore no less a spherical wave with
velocity of propagation c when viewed in the moving system. This shows that
our two fundamental principles are compatible.5
In the equations of transformation which have been developed there enters
an unknown function φ of v, which we will now determine.
For this purpose we introduce a third system of co-ordinates K0 , which rela-
tively to the system k is in a state of parallel translatory motion parallel to the
axis of X, such that the origin of co-ordinates of system k moves with velocity
−v on the axis of X. At the time t = 0 let all three origins coincide, and when
t = x = y = z = 0 let the time t0 of the system K0 be zero. We call the coordinates, measured in the system K0 , x0 , y 0 , z 0 , and by a twofold application of our equations of transformation we obtain
t0
x0
y0
z0
=
=
=
=
φ(−v)β(−v)(τ + vξ/c2 )
φ(−v)β(−v)(ξ + vτ )
φ(−v)η
φ(−v)ζ
=
=
=
=
φ(v)φ(−v)t,
φ(v)φ(−v)x,
φ(v)φ(−v)y,
φ(v)φ(−v)z.
Since the relations between x0 , y 0 , z 0 and x, y, z do not contain the time t,
the systems K and K0 are at rest with respect to one another, and it is clear that
the transformation from K to K0 must be the identical transformation. Thus
φ(v)φ(−v) = 1.

We now inquire into the signification of φ(v). We give our attention to that
part of the axis of Y of system k which lies between ξ = 0, η = 0, ζ = 0 and
ξ = 0, η = l, ζ = 0. This part of the axis of Y is a rod moving perpendicularly
5 The equations of the Lorentz transformation may be more simply deduced directly from
the condition that in virtue of those equations the relation x2 + y 2 + z 2 = c2 t2 shall have as
its consequence the second relation ξ 2 + η2 + ζ 2 = c2 τ 2 .
8to its axis with velocity v relatively to system K. Its ends possess in K the
co-ordinates
x1 = vt, y1 =
l
, z1 = 0
φ(v)
and
x2 = vt, y2 = 0, z2 = 0.
The length of the rod measured in K is therefore l/φ(v); and this gives us the
meaning of the function φ(v). From reasons of symmetry it is now evident that
the length of a given rod moving perpendicularly to its axis, measured in the
stationary system, must depend only on the velocity and not on the direction
and the sense of the motion. The length of the moving rod measured in the
stationary system does not change, therefore, if v and −v are interchanged.
Hence follows that l/φ(v) = l/φ(−v), or
φ(v) = φ(−v).

It follows from this relation and the one previously found that φ(v) = 1, so that
the transformation equations which have been found become
τ
ξ= β(t − vx/c2 ),
= β(x − vt),
η
ζ= y,
= z,
where
p
β = 1/ 1 − v 2 /c2 .

